@prefix : <http://lod.nik.uni-obuda.hu/iloc/iloc#> .
@prefix vs: <http://www.w3.org/2003/06/sw-vocab-status/ns#> .
@prefix geo: <http://www.w3.org/2003/01/geo/wgs84_pos#> .
@prefix owl: <http://www.w3.org/2002/07/owl#> .
@prefix rdf: <http://www.w3.org/1999/02/22-rdf-syntax-ns#> .
@prefix xml: <http://www.w3.org/XML/1998/namespace> .
@prefix xsd: <http://www.w3.org/2001/XMLSchema#> .
@prefix foaf: <http://xmlns.com/foaf/0.1/> .
@prefix rdfs: <http://www.w3.org/2000/01/rdf-schema#> .
@prefix vann: <http://purl.org/vocab/vann/> .
@prefix teach: <http://linkedscience.org/teach/ns#> .
@prefix vcard: <http://www.w3.org/2006/vcard/ns#> .
@prefix dcterm: <http://purl.org/dc/terms/> .
@base <http://lod.nik.uni-obuda.hu/iloc/iloc#> .

<http://lod.nik.uni-obuda.hu/iloc/iloc#> rdf:type owl:Ontology ;
                                         
                                         dcterm:issued "2015-07-01"^^xsd:date ;
                                         
                                         dcterm:date "2016-10-28"^^xsd:date ;
                                         
                                         dcterm:identifier "http://lod.nik.uni-obuda.hu/iloc-20161028" ;
                                         
                                         vann:preferredNamespacePrefix "iloc" ;
                                         
                                         dcterm:isVersionOf "http://lod.nik.uni-obuda.hu/iloc/iloc#" ;
                                         
                                         vann:preferredNamespaceUri "http://lod.nik.uni-obuda.hu/iloc/iloc#" ;
                                         
                                         dcterm:title "Ontology for Indoor Navigation" ;
                                         
                                         dcterm:description "This ontology provides indoor location and navigation features."@en ;
                                         
                                         <http://creativecommons.org/ns#license> <http://creativecommons.org/licenses/by/3.0/> ;
                                         
                                         dcterm:creator <http://lod.nik.uni-obuda.hu/data/Andras_Micsik> ,
                                                        <http://lod.nik.uni-obuda.hu/data/Barnabas_Szasz> ,
                                                        <http://lod.nik.uni-obuda.hu/data/Rita_Fleiner> ;
                                         
                                         owl:imports <http://www.w3.org/2006/vcard/ns> .


#################################################################
#
#    Annotation properties
#
#################################################################


###  http://purl.org/dc/elements/1.1/date

<http://purl.org/dc/elements/1.1/date> rdf:type owl:AnnotationProperty .



###  http://purl.org/dc/elements/1.1/description

<http://purl.org/dc/elements/1.1/description> rdf:type owl:AnnotationProperty .



###  http://purl.org/dc/elements/1.1/title

<http://purl.org/dc/elements/1.1/title> rdf:type owl:AnnotationProperty .


#################################################################
#
#    Object Properties
#
#################################################################


###  http://lod.nik.uni-obuda.hu/iloc/iloc#belongsTo

:belongsTo rdf:type owl:ObjectProperty ;
           
           rdfs:label "belongs to"@en ;
           
           rdfs:comment "This property can be used to state that a Room belongs to a specific Organization or Person."@en ;
           
           vs:term_status "stable"@en ;
           
           rdfs:domain :Room ;
           
           rdfs:range foaf:Agent .



###  http://lod.nik.uni-obuda.hu/iloc/iloc#belongsToRoom

:belongsToRoom rdf:type owl:ObjectProperty ;
               
               rdfs:label "belongs to Room"@en ;
               
               rdfs:comment "This property states that a Point of Interest belongs to a Room. POIs can belong to multiple rooms: e.g. doors are part of both rooms." ;
               
               vs:term_status "stable"@en ;
               
               rdfs:domain :POI ;
               
               rdfs:range :Room .



###  http://lod.nik.uni-obuda.hu/iloc/iloc#connectsPOI

:connectsPOI rdf:type owl:ObjectProperty ,
                      owl:SymmetricProperty ;
             
             rdfs:label "connects to POI"@en ;
             
             rdfs:comment "This property is used to describe a direct route between POIs."@en ;
             
             vs:term_status "stable"@en ;
             
             rdfs:range :POI ;
             
             rdfs:domain :POI ;
             
             rdfs:subPropertyOf :connectsPOIOneWay .



###  http://lod.nik.uni-obuda.hu/iloc/iloc#connectsPOIOneWay

:connectsPOIOneWay rdf:type owl:AsymmetricProperty ,
                            owl:ObjectProperty ;
                   
                   rdfs:label "connects to POI (one way)"@en ;
                   
                   rdfs:comment "This property is used to describe a direct walkable one-way route between POIs. Only walking from the subject to the object is possible/allowed."@en ;
                   
                   vs:term_status "stable"@en ;
                   
                   rdfs:range :POI ;
                   
                   rdfs:domain :POI .



###  http://lod.nik.uni-obuda.hu/iloc/iloc#defaultRoomOf

:defaultRoomOf rdf:type owl:ObjectProperty ;
               
               rdfs:label "default Room Of"@en ;
               
               rdfs:comment "This property assigns a default Room to an Organization or Person."@en ;
               
               vs:term_status "stable"@en ;
               
               rdfs:range :Room ;
               
               rdfs:domain foaf:Agent .



###  http://lod.nik.uni-obuda.hu/iloc/iloc#hasCategory

:hasCategory rdf:type owl:ObjectProperty ;
             
             rdfs:label "has Category"@en ;
             
             rdfs:comment "This property states that a Room or Point of Interest has a specific category, like Hallway, Office, etc. Category can be any resource." ;
             
             vs:term_status "stable"@en .



###  http://lod.nik.uni-obuda.hu/iloc/iloc#hasEntrance

:hasEntrance rdf:type owl:ObjectProperty ;
             
             rdfs:label "has Entrance"@en ;
             
             rdfs:comment "This property states that an Entrance belongs to a Room. Entrances belong to multiple rooms." ;
             
             vs:term_status "stable"@en ;
             
             rdfs:domain :Entrance ;
             
             rdfs:range :Room ;
             
             rdfs:subPropertyOf :belongsToRoom .



###  http://lod.nik.uni-obuda.hu/iloc/iloc#hasPOI

:hasPOI rdf:type owl:ObjectProperty ;
        
        rdfs:label "has POI"@en ;
        
        rdfs:comment "This property states that there is a Point of Interest in a Room. Multiple rooms can include the same POI: e.g. doors are part of both rooms."@en ;
        
        vs:term_status "stable"@en ;
        
        rdfs:range :POI ;
        
        rdfs:domain :Room ;
        
        owl:inverseOf :belongsToRoom .



###  http://lod.nik.uni-obuda.hu/iloc/iloc#hasPart

:hasPart rdf:type owl:ObjectProperty ;
         
         rdfs:label "has part"@en ;
         
         rdfs:comment "Object property to state that a Building or BuildingPart has a BuildingPart. Example: ex:buildingA iloc:hasPart ex:Floor1_buildingA ."@en ;
         
         vs:term_status "stable"@en ;
         
         rdfs:domain :BuildingPart ;
         
         rdfs:range [ rdf:type owl:Class ;
                      owl:unionOf ( :Building
                                    :BuildingPart
                                  )
                    ] .



###  http://lod.nik.uni-obuda.hu/iloc/iloc#hasRouteFeature

:hasRouteFeature rdf:type owl:ObjectProperty ;
                 
                 rdfs:label "has Route Feature"@en ;
                 
                 rdfs:comment "This property states that a RouteSection has a specific feature." ;
                 
                 vs:term_status "stable"@en ;
                 
                 rdfs:domain :RouteFeature ;
                 
                 rdfs:range :RouteSection .



###  http://lod.nik.uni-obuda.hu/iloc/iloc#isPartOf

:isPartOf rdf:type owl:ObjectProperty ;
          
          rdfs:label "is part of"@en ;
          
          rdfs:comment "Object property to state that a BuildingPart entity is part of a Building or BuildingPart. Example: ex:Floor1_buildingA iloc:isPartOf ex:buildingA ."@en ;
          
          vs:term_status "stable"@en ;
          
          rdfs:domain :BuildingPart ;
          
          owl:inverseOf :hasPart ;
          
          rdfs:range [ rdf:type owl:Class ;
                       owl:unionOf ( :Building
                                     :BuildingPart
                                   )
                     ] .



###  http://lod.nik.uni-obuda.hu/iloc/iloc#routeFromPOI

:routeFromPOI rdf:type owl:ObjectProperty ;
              
              rdfs:label "connects to RouteSection"@en ;
              
              rdfs:comment "This property is used to define the start POI of a RouteSection instance."@en ;
              
              vs:term_status "stable"@en ;
              
              rdfs:range :POI ;
              
              rdfs:domain :RouteSection ;
              
              rdfs:subPropertyOf :routeToFromPOI .



###  http://lod.nik.uni-obuda.hu/iloc/iloc#routeToFromPOI

:routeToFromPOI rdf:type owl:ObjectProperty ;
                
                rdfs:label "connects to RouteSection"@en ;
                
                rdfs:comment "This property is used to define either one of the POIs of a RouteSection instance."@en ;
                
                vs:term_status "stable"@en ;
                
                rdfs:range :POI ;
                
                rdfs:domain :RouteSection .



###  http://lod.nik.uni-obuda.hu/iloc/iloc#routeToPOI

:routeToPOI rdf:type owl:ObjectProperty ;
            
            rdfs:label "connects to RouteSection"@en ;
            
            rdfs:comment "This property is used to define the target POI of a RouteSection instance."@en ;
            
            vs:term_status "stable"@en ;
            
            rdfs:range :POI ;
            
            rdfs:domain :RouteSection ;
            
            rdfs:subPropertyOf :routeToFromPOI .



###  http://www.w3.org/2003/01/geo/wgs84_pos#location

geo:location rdf:type owl:ObjectProperty ;
             
             rdfs:range geo:SpatialThing .





#################################################################
#
#    Classes
#
#################################################################


###  http://lod.nik.uni-obuda.hu/iloc/iloc#Building

:Building rdf:type owl:Class ;
          
          rdfs:label "Building"@en ;
          
          rdfs:subClassOf owl:Thing ,
                          [ rdf:type owl:Restriction ;
                            owl:onProperty :hasEntrance ;
                            owl:minCardinality "1"^^xsd:nonNegativeInteger
                          ] ,
                          [ rdf:type owl:Restriction ;
                            owl:onProperty :hasPart ;
                            owl:allValuesFrom :Floor
                          ] ;
          
          rdfs:comment "Represents a whole building. It may have an address and spatial coordinates."@en ;
          
          vs:term_status "stable"@en .



###  http://lod.nik.uni-obuda.hu/iloc/iloc#BuildingEntrance

:BuildingEntrance rdf:type owl:Class ;
                  
                  rdfs:label "Building Entrance"@en ;
                  
                  rdfs:subClassOf :Entrance ,
                                  [ rdf:type owl:Restriction ;
                                    owl:onProperty :belongsToRoom ;
                                    owl:maxCardinality "1"^^xsd:nonNegativeInteger
                                  ] ;
                  
                  rdfs:comment "Represents the entrance where one can enter/leave the building."@en ;
                  
                  vs:term_status "stable"@en .



###  http://lod.nik.uni-obuda.hu/iloc/iloc#BuildingPart

:BuildingPart rdf:type owl:Class ;
              
              rdfs:label "Building Part"@en ;
              
              rdfs:subClassOf owl:Thing ;
              
              rdfs:comment "Superclass of every part of a building."@en ;
              
              vs:term_status "stable"@en .



###  http://lod.nik.uni-obuda.hu/iloc/iloc#Distance

:Distance rdf:type owl:Class ;
          
          rdfs:label "distance"@en ;
          
          rdfs:subClassOf :QuantityRouteFeature ;
          
          rdfs:comment "Distance instances represent the time or distance it is take to traverse a Route Section."@en ;
          
          vs:term_status "stable"@en .



###  http://lod.nik.uni-obuda.hu/iloc/iloc#Elevator

:Elevator rdf:type owl:Class ;
          
          rdfs:label "Elevator"@en ;
          
          rdfs:subClassOf :VerticalPassage ;
          
          rdfs:comment "Connects Rooms on different floors."@en ;
          
          vs:term_status "stable"@en .



###  http://lod.nik.uni-obuda.hu/iloc/iloc#Entrance

:Entrance rdf:type owl:Class ;
          
          rdfs:label "Entrance"@en ;
          
          rdfs:subClassOf :POI ,
                          [ rdf:type owl:Restriction ;
                            owl:onProperty :belongsToRoom ;
                            owl:maxCardinality "2"^^xsd:nonNegativeInteger
                          ] ;
          
          rdfs:comment "Represents any type of entrance"@en ;
          
          vs:term_status "stable"@en .



###  http://lod.nik.uni-obuda.hu/iloc/iloc#Floor

:Floor rdf:type owl:Class ;
       
       rdfs:label "Floor"@en ;
       
       rdfs:subClassOf :BuildingPart ,
                       [ rdf:type owl:Restriction ;
                         owl:onProperty :hasPart ;
                         owl:allValuesFrom :Room
                       ] ;
       
       rdfs:comment "It is part of a building. It may consist of Rooms."@en ;
       
       vs:term_status "stable"@en .



###  http://lod.nik.uni-obuda.hu/iloc/iloc#FunctionalRouteFeature

:FunctionalRouteFeature rdf:type owl:Class ;
                        
                        rdfs:label "Functional Route feature"@en ;
                        
                        rdfs:subClassOf :RouteFeature ;
                        
                        rdfs:comment "FunctionalRouteFeature instances represent any functional feature a Route Section might have."@en ;
                        
                        vs:term_status "stable"@en .



###  http://lod.nik.uni-obuda.hu/iloc/iloc#HasIncline

:HasIncline rdf:type owl:Class ;
            
            rdfs:label "Has Incline"@en ;
            
            rdfs:subClassOf :QualityRouteFeature ;
            
            rdfs:comment "A Route Section has incline (in degrees)."@en ;
            
            vs:term_status "stable"@en .



###  http://lod.nik.uni-obuda.hu/iloc/iloc#HasSteps

:HasSteps rdf:type owl:Class ;
          
          rdfs:label "Has Steps"@en ;
          
          rdfs:subClassOf :QualityRouteFeature ;
          
          rdfs:comment "A Route Section has steps."@en ;
          
          vs:term_status "stable"@en .



###  http://lod.nik.uni-obuda.hu/iloc/iloc#POI

:POI rdf:type owl:Class ;
     
     rdfs:label "Point of Interest"@en ;
     
     rdfs:subClassOf owl:Thing ;
     
     rdfs:comment "An entity with Location. Can be used as part of a route."@en ;
     
     vs:term_status "stable"@en .



###  http://lod.nik.uni-obuda.hu/iloc/iloc#QualityRouteFeature

:QualityRouteFeature rdf:type owl:Class ;
                     
                     rdfs:label "Quality Route feature"@en ;
                     
                     rdfs:subClassOf :RouteFeature ;
                     
                     rdfs:comment "QualityRouteFeature instances represent any quality feature a Route Section might have."@en ;
                     
                     vs:term_status "stable"@en .



###  http://lod.nik.uni-obuda.hu/iloc/iloc#QuantityRouteFeature

:QuantityRouteFeature rdf:type owl:Class ;
                      
                      rdfs:label "Quantitiv Route feature"@en ;
                      
                      rdfs:subClassOf :RouteFeature ;
                      
                      rdfs:comment "QuantityRouteFeature instances represent any quantive feature a Route Section might have."@en ;
                      
                      vs:term_status "stable"@en .



###  http://lod.nik.uni-obuda.hu/iloc/iloc#Room

:Room rdf:type owl:Class ;
      
      rdfs:label "Room"@en ;
      
      rdfs:subClassOf :BuildingPart ,
                      [ rdf:type owl:Restriction ;
                        owl:onProperty :hasEntrance ;
                        owl:minCardinality "1"^^xsd:nonNegativeInteger
                      ] ;
      
      rdfs:comment "Represents any type of room within a building."@en ;
      
      vs:term_status "stable"@en ;
      
      rdfs:isDefinedBy <http://yago-knowledge.org/resource/wordnet_room_104105893> .



###  http://lod.nik.uni-obuda.hu/iloc/iloc#RoomEntrance

:RoomEntrance rdf:type owl:Class ;
              
              rdfs:label "Room Entrance"@en ;
              
              rdfs:subClassOf :Entrance ;
              
              rdfs:comment "Represents the entrance where one can enter/leave the room."@en ;
              
              vs:term_status "stable"@en .



###  http://lod.nik.uni-obuda.hu/iloc/iloc#RouteFeature

:RouteFeature rdf:type owl:Class ;
              
              rdfs:label "Route feature"@en ;
              
              rdfs:comment "RouteFeature instances represent any feature a Route Section might have."@en ;
              
              vs:term_status "stable"@en .



###  http://lod.nik.uni-obuda.hu/iloc/iloc#RouteSection

:RouteSection rdf:type owl:Class ;
              
              rdfs:label "Route section"@en ;
              
              rdfs:comment "Route section directly connecting two POIs"@en ;
              
              vs:term_status "stable"@en .



###  http://lod.nik.uni-obuda.hu/iloc/iloc#Stairway

:Stairway rdf:type owl:Class ;
          
          rdfs:label "Stairway"@en ;
          
          rdfs:subClassOf :VerticalPassage ;
          
          rdfs:comment "Connects Rooms on different floors."@en ;
          
          vs:term_status "stable"@en .



###  http://lod.nik.uni-obuda.hu/iloc/iloc#VerticalPassage

:VerticalPassage rdf:type owl:Class ;
                 
                 rdfs:label "VerticalPassage"@en ;
                 
                 rdfs:subClassOf :Room ;
                 
                 rdfs:comment "Connects Rooms on different floors using any method."@en ;
                 
                 vs:term_status "stable"@en .



###  http://www.w3.org/2003/01/geo/wgs84_pos#Point

geo:Point rdf:type owl:Class ;
          
          rdfs:label "point" ;
          
          rdfs:subClassOf geo:SpatialThing ;
          
          rdfs:comment """ 
Uniquely identified by lat/long/alt. i.e.

spaciallyIntersects(P1, P2) :- lat(P1, LAT), long(P1, LONG), alt(P1, ALT),
  lat(P2, LAT), long(P2, LONG), alt(P2, ALT).

sameThing(P1, P2) :- type(P1, Point), type(P2, Point), spaciallyIntersects(P1, P2).
  """ ,
                       """A point, typically described using a coordinate system relative to Earth, such as WGS84.
  """ .



###  http://www.w3.org/2003/01/geo/wgs84_pos#SpatialThing

geo:SpatialThing rdf:type owl:Class ;
                 
                 rdfs:label "SpatialThing" ;
                 
                 rdfs:comment """Anything with spatial extent, i.e. size, shape, or position.
 e.g. people, places, bowling balls, as well as abstract areas like cubes.
""" .



###  http://xmlns.com/foaf/0.1/Agent

foaf:Agent rdf:type owl:Class .




#################################################################
#
#    Individuals
#
#################################################################

###  http://lod.nik.uni-obuda.hu/iloc/iloc#Wheelchair
:Wheelchair rdf:type :AccessFeature ,
             owl:NamedIndividual ;
				   
			rdfs:label "Wheelchair"@en ;
                              
            vs:term_status "stable"@en ;
          
            rdfs:comment "Provides access for people with a disability being tied to a wheelchair."@en .			

###  http://lod.nik.uni-obuda.hu/iloc/iloc#EWheelchair
:EWheelchair rdf:type :AccessFeature ,
             owl:NamedIndividual ;
				   
			rdfs:label "Electronic Wheelchair"@en ;
                              
            vs:term_status "stable"@en ;
          
            rdfs:comment "Provides access for people with a disability being tied to an electronic wheelchair."@en .			

###  http://lod.nik.uni-obuda.hu/iloc/iloc#WheelchairWHelp
:WheelchairWHelp rdf:type :AccessFeature ,
             owl:NamedIndividual ;
				   
			rdfs:label "Wheelchair with Help"@en ;
                              
            vs:term_status "stable"@en ;
          
            rdfs:comment "Provides access for people with a disability being tied to a wheelchair with some additional help."@en .			

###  http://lod.nik.uni-obuda.hu/iloc/iloc#Stretcher
:Stretcher rdf:type :AccessFeature ,
             owl:NamedIndividual ;
				   
			rdfs:label "Stretcher"@en ;
                              
            vs:term_status "stable"@en ;
          
            rdfs:comment "Provides access for people pushing a stretcher."@en .			

###  http://lod.nik.uni-obuda.hu/iloc/iloc#RestrictedAccess
:RestrictedAccess rdf:type :AccessFeature ,
             owl:NamedIndividual ;
				   
			rdfs:label "Restricted Access"@en ;
                              
            vs:term_status "stable"@en ;
          
            rdfs:comment "It represents restricted access to part of a building, for example the need for having an employee badge."@en .			

###  http://lod.nik.uni-obuda.hu/iloc/iloc#Stroller
:Stroller rdf:type :AccessFeature ,
             owl:NamedIndividual ;
				   
			rdfs:label "Stroller"@en ;
                              
            vs:term_status "stable"@en ;
          
            rdfs:comment "Provides access for people with a stroller."@en .			


#################################################################
#
#    Annotations
#
#################################################################


###  Generated by the OWL API (version 3.5.1) http://owlapi.sourceforge.net

